formalization/thesis/Isotope/LambdaCase.lean
@@ -2,5 +2,8 @@ import Isotope.LambdaCase.Syntax
 import Isotope.LambdaCase.Typing
 import Isotope.LambdaCase.TypingSubst
 import Isotope.LambdaCase.Equiv
+import Isotope.LambdaCase.Semantics
 import Isotope.LambdaCase.Semantics.Categorical
+import Isotope.LambdaCase.Semantics.Identity
+import Isotope.LambdaCase.Semantics.Substitution
 import Isotope.LambdaCase.Subtyping
